

Theorem 0.0.1. Suppose X and Y are independent random variables with

$$f_X(x) = \frac{1}{2\pi} e^{-\frac{1}{2}(x^2+y^2)} \quad \text{for } x \in \mathbb{R}$$

and $Y \sim \chi_\nu^2$, that is

$$f_Y(y) = \frac{1}{2^{\nu/2} \Gamma(\nu/2)} y^{\nu/2-1} e^{-y/2}$$

Then the random variable T defined by

$$T := \frac{X}{\sqrt{Y/\nu}}$$

follows Student's t -distribution with ν degrees of freedom.

Proof. Let T be defined as above and define $Z := \sqrt{Y/\nu}$. Then we have $x(t, z) = tz$ and $y(t, z) = \nu z^2$. We also compute the partial derivatives as

$$\frac{\partial x}{\partial t} = z \quad \frac{\partial x}{\partial z} = t \quad \frac{\partial y}{\partial t} = 0 \quad \frac{\partial y}{\partial z} = 2\nu z$$

Recalling the formula for the transformation of random variables, we can write

$$f_{T,Z}(t, z) = f_{X,Y}(x(t, z), y(t, z)) |J(t, z)|$$

where $J(t, z)$ is the Jacobian matrix. To start off, we compute the Jacobian as

$$\begin{vmatrix} z & t \\ 0 & 2\nu z \end{vmatrix} = 2\nu z^2$$

and, noting that $\nu \in \mathbb{N}$, we conclude $|J| = 2\nu z^2$.

Therefore,

$$\begin{aligned} f_{T,Z} &= f_X(x(t, z)) f_Y(y(t, z)) |J| && \text{(by independence)} \\ &= \frac{\frac{1}{\sqrt{2\pi}} e^{-\frac{1}{2}t^2 z^2} (\nu z^2)^{\nu/2-1} e^{-\frac{1}{2}\nu z^2} (2\nu z^2)}{2^{\nu/2} \Gamma(\nu/2)} \\ &= \frac{\nu^{\nu/2} z^\nu e^{-\frac{1}{2}t^2 z^2} e^{-\frac{1}{2}\nu z^2}}{2^{\frac{1}{2}(1-\nu)} \Gamma(\nu/2) \sqrt{\pi}} \end{aligned}$$

To obtain the pdf of T we compute the marginal. Note that z ranges from 0 to $+\infty$.

$$f_T(t) = \frac{\nu^{\nu/2}}{2^{\frac{1}{2}(1-\nu)} \Gamma(\nu/2) \sqrt{\pi}} \underbrace{\int_0^\infty z^\nu e^{\frac{1}{2}(z^2(t^2+\nu))} dz}_I$$

To evaluate I we change the variable to $\gamma := \frac{1}{2}(z^2(t^2 + \nu))$, so that

$$z = \left(\frac{2\gamma}{t^2 + \nu} \right)^{1/2} \quad \text{and} \quad dz = \frac{d\gamma}{z(t^2 + \nu)}$$

Therefore

$$\begin{aligned} I &= \int_0^\infty \left(\frac{2\gamma}{t^2 + \nu} \right)^{\nu/2} e^{-\gamma} \frac{d\gamma}{\left(\frac{2\gamma}{t^2 + \nu} \right)^{1/2} (t^2 + \nu)} \\ &= \int_0^\infty \left(\frac{2\gamma}{t^2 + \nu} \right)^{\nu/2} e^{-\gamma} \frac{1}{\sqrt{2}\gamma^{1/2}(t^2 + \nu)} d\gamma \\ &= \sqrt{2}^{\nu-1} (t^2 + \nu)^{-\frac{\nu+1}{2}} \int_0^\infty \gamma^{\frac{\nu-1}{2}} e^{-\gamma} d\gamma \\ &= \sqrt{2}^{\nu-1} (t^2 + \nu)^{-\frac{\nu+1}{2}} \int_0^\infty \gamma^{\frac{\nu+1}{2}-1} e^{-\gamma} d\gamma = \sqrt{2}^{\nu-1} (t^2 + \nu)^{-\frac{\nu+1}{2}} \Gamma\left(\frac{\nu+1}{2}\right) \end{aligned}$$

Putting this together,

$$\begin{aligned}
 f_T(t) &= \frac{\cancel{2^{\frac{1}{2}(\nu+1)}} \nu^{\nu/2} (t^2 + \nu)^{\frac{1}{2}(\nu+1)}}{\cancel{2^{\frac{1}{2}(1-\nu)}} \Gamma(\nu/2) \sqrt{\pi}} \Gamma\left(\frac{\nu+1}{2}\right) \\
 &= \frac{\nu^{\cancel{\nu/2}} \left(\frac{t^2}{\nu} + 1\right)^{\frac{1}{2}(\nu+1)}}{\Gamma(\nu/2) \sqrt{\pi} \cancel{\nu^{\nu/2}} \sqrt{\nu}} \Gamma\left(\frac{\nu+1}{2}\right) \\
 &= \frac{\Gamma\left(\frac{\nu+1}{2}\right)}{\sqrt{\nu\pi} \Gamma(\nu/2)} \left(\frac{t^2}{\nu} + 1\right)^{\frac{\nu+1}{2}}
 \end{aligned}$$

This is exactly the pdf of Student's t -distribution with ν degrees of freedom. □